map_of_list_pair: FE-ize equality tests

src/cddl/spec/CDDL.Spec.AST.Base.fst
@@ -1,4 +1,5 @@
 module CDDL.Spec.AST.Base
+include CDDL.Spec.EqTest
 module Spec = CDDL.Spec.All
 module U64 = FStar.UInt64
 module Cbor = CBOR.Spec.API.Type
@@ -2374,33 +2375,6 @@ let target_type_sem_rec
   (t: target_type { target_type_positively_bounded (extend_name_env bound new_name NType) bound t })
 : GTot Type0
 = rectype (target_type_sem_rec_body bound env new_name s t)
-
-module FE = FStar.FunctionalExtensionality
-
-let eq_test (t: Type) : Type =
-  FE.restricted_t t (fun x1 -> FE.restricted_t t (fun x2 -> (y: bool { y == true <==> x1 == x2 })))
-
-let feq2 (#t1 #t2 #t: Type) (f g: (t1 -> t2 -> t)) : Tot prop =
-  forall x1 x2 . f x1 x2 == g x1 x2
-
-let feq_intro
-  (#t: Type)
-  (#t': t -> Type)
-  (f1 f2: FE.restricted_t t t')
-  (prf: (x: t) -> Lemma
-    (f1 x == f2 x)
-  )
-: Lemma
-  (f1 == f2)
-= Classical.forall_intro prf;
-  assert (FE.feq f1 f2)
-
-let eq_test_unique (#t: Type) (f1 f2: eq_test t) : Lemma
-  (f1 == f2)
-= feq_intro f1 f2 (fun x -> feq_intro (f1 x) (f2 x) (fun _ -> ()))
-
-let mk_eq_test (#t: Type) (phi: ((x1: t) -> (x2: t) -> Pure bool True (fun res -> res == true <==> x1 == x2))) : Tot (eq_test t) =
-  FE.on_dom t (fun x1 -> FE.on_dom t (fun x2 -> phi x1 x2 <: (y: bool { y == true <==> x1 == x2 })))
 
 noextract
 noeq type target_type_env
